progs/verif_nest2.v
@@ -32,30 +32,9 @@ Definition Gprog : funspecs :=
 
 Lemma body_get:  semax_body Vprog Gprog f_get get_spec.
 Proof.
- start_function.
+start_function.
 name i _i.
-apply (remember_value (eval_var _p t_struct_b)); intro p.
-eapply semax_seq'.
-
-ensure_normal_ret_assert;
- hoist_later_in_pre.
-change (Efield (Efield (Evar _p t_struct_b) _y2 t_struct_a) _x2 tint)
- with (nested_efield (Evar _p t_struct_b) (_x2 :: _y2 :: nil) (tint :: t_struct_a :: nil)).
-eapply semax_nested_efield_load_37'.
-reflexivity.
-reflexivity.
-instantiate (1 := Struct_env). reflexivity.
-reflexivity.
-reflexivity.
-reflexivity.
-reflexivity.
-entailer!.
-simpl; auto.
-
-unfold replace_nth; cbv beta;
-               try (apply extract_exists_pre; intro_old_var (Sset _i (Efield (Efield (Evar _p t_struct_b) _y2 t_struct_a) _x2 tint)));
-               abbreviate_semax.
-
+forward.
 simpl proj_reptype.
 forward.
 apply derives_refl.
@@ -65,32 +44,7 @@ Lemma body_set:  semax_body Vprog Gprog f_set set_spec.
 Proof.
  start_function.
 name i_ _i.
-apply (remember_value (eval_var _p t_struct_b)); intro p.
-
-eapply semax_seq'.
-
-ensure_normal_ret_assert;
- hoist_later_in_pre.
-change (Efield (Efield (Evar _p t_struct_b) _y2 t_struct_a) _x2 tint)
- with (nested_efield (Evar _p t_struct_b) (_x2 :: _y2 :: nil) (tint :: t_struct_a :: nil)).
-
-eapply semax_nested_efield_store_nth with (n := 0%nat).
-reflexivity.
-reflexivity.
-instantiate (1 := Struct_env). reflexivity.
-reflexivity.
-reflexivity.
-reflexivity.
-reflexivity.
-entailer!.
-auto.
-entailer!.
-
-unfold replace_nth; cbv beta;
-               try (apply extract_exists_pre; intro_old_var (Sassign (Efield (Efield (Evar _p t_struct_b) _y2 t_struct_a) _x2 tint)
-        (Etempvar _i tint)));
-               abbreviate_semax.
-
+forward.
 forward.
 entailer!.
 Qed.
