progs/verif_nest3.v
@@ -34,31 +34,16 @@ Lemma body_get:  semax_body Vprog Gprog f_get get_spec.
 Proof.
  start_function.
 name i _i.
-apply (remember_value (eval_var _p t_struct_c)); intro p.
-simpl_data_at.
 forward.
-Admitted.
-(*
 forward.
-simpl_data_at.
 cancel.
 Qed.
-*)
 
 Lemma body_set:  semax_body Vprog Gprog f_set set_spec.
 Proof.
- start_function.
+start_function.
 name i_ _i.
-apply (remember_value (eval_var _p t_struct_c)); intro p.
-simpl_data_at.
-Admitted.
-(*
 forward.
 forward.
-unfold at_offset, id; simpl.
-forget (eval_var _p t_struct_c rho) as p.
-simpl_data_at.
-fold t_struct_a.
 cancel.
 Qed.
-*)
